benchmarks/benchmark.c
@@ -1105,6 +1105,7 @@ void call_mldsa_ntt(void) repeat(mldsa_ntt((int32_t*)b0,(const int32_t*)b1))
 void call_mldsa_pointwise(void) repeat(mldsa_pointwise_x86((int32_t*)b0,(int32_t*)b1,(int32_t*)b2,(int32_t*)b3))
 void call_mldsa_pointwise_acc_l4(void) repeat(mldsa_pointwise_acc_l4_x86((int32_t*)b0,(const int32_t*)b1,(const int32_t*)b2,mldsa_avx2_qdata))
 void call_mldsa_pointwise_acc_l5(void) repeat(mldsa_pointwise_acc_l5_x86((int32_t*)b0,(const int32_t*)b1,(const int32_t*)b2,mldsa_avx2_qdata))
+void call_mldsa_pointwise_acc_l7(void) repeat(mldsa_pointwise_acc_l7_x86((int32_t*)b0,(const int32_t*)b1,(const int32_t*)b2,mldsa_avx2_qdata))
 void call_mldsa_reduce(void) repeat(mldsa_reduce((int32_t*)b0))
 
 void call_mlkem_frombytes(void) repeat(mlkem_frombytes((uint16_t*)b0,(int8_t*)b1))
@@ -1133,6 +1134,7 @@ void call_mldsa_ntt(void) {}
 void call_mldsa_pointwise(void) repeat(mldsa_pointwise((int32_t*)b0,(int32_t*)b1,(int32_t*)b2))
 void call_mldsa_pointwise_acc_l4(void) repeat(mldsa_pointwise_acc_l4((int32_t*)b0,(const int32_t*)b1,(const int32_t*)b2))
 void call_mldsa_pointwise_acc_l5(void) repeat(mldsa_pointwise_acc_l5((int32_t*)b0,(const int32_t*)b1,(const int32_t*)b2))
+void call_mldsa_pointwise_acc_l7(void) repeat(mldsa_pointwise_acc_l7((int32_t*)b0,(const int32_t*)b1,(const int32_t*)b2))
 void call_mldsa_reduce(void) {}
 
 void call_bignum_copy_row_from_table_8n__32_16(void) \
@@ -1557,6 +1559,7 @@ int main(int argc, char *argv[])
   timingtest(all,"mldsa_pointwise",call_mldsa_pointwise);
   timingtest(all,"mldsa_pointwise_acc_l4",call_mldsa_pointwise_acc_l4);
   timingtest(all,"mldsa_pointwise_acc_l5",call_mldsa_pointwise_acc_l5);
+  timingtest(all,"mldsa_pointwise_acc_l7",call_mldsa_pointwise_acc_l7);
   timingtest(!arm,"mldsa_reduce",call_mldsa_reduce);
   timingtest(bmi,"p256_montjadd",call_p256_montjadd);
   timingtest(all,"p256_montjadd_alt",call_p256_montjadd_alt);
